added sstack_val comparator with equality check, both implementation and soundness proof

sstack_val_cmp_impl.v
@@ -134,6 +134,75 @@ Fixpoint basic_compare_sstack_val (smemory_cmp: smemory_cmp_ext_t) (sstorage_cmp
       end
   end.
 
+Fixpoint basic_compare_sstack_val_w_eq_chk (smemory_cmp: smemory_cmp_ext_t) (sstorage_cmp: sstorage_cmp_ext_t) (sha3_cmp: sha3_cmp_ext_t) (d: nat) (ctx: constraints) (sv1 sv2: sstack_val) (maxidx1: nat) (sb1: sbindings) (maxidx2: nat) (sb2: sbindings) (ops: stack_op_instr_map) : bool :=
+  if (trivial_compare_sstack_val smemory_cmp sstorage_cmp sha3_cmp d ctx sv1 sv2 maxidx1 sb1 maxidx2 sb2 ops)
+  then true
+  else
+  match d with
+  | 0 => false
+  | S d' =>
+      let basic_compare_sstack_val_w_eq_chk_rec :=
+        basic_compare_sstack_val_w_eq_chk smemory_cmp sstorage_cmp sha3_cmp d' in
+      match follow_in_smap sv1 maxidx1 sb1 with
+      | None => false
+      | Some (FollowSmapVal smv1 maxidx1' sb1') =>
+          match  follow_in_smap sv2 maxidx2 sb2 with
+          | None => false
+          | Some (FollowSmapVal smv2 maxidx2' sb2') =>
+              match smv1, smv2 with 
+              | SymBasicVal sv1', SymBasicVal sv2' =>
+                  match sv1',sv2' with
+                  | Val w1, Val w2 => weqb w1 w2
+                  | InVar n1, InVar n2 => (n1 =? n2)
+                  | _, _ => false
+                  end
+              | SymMETAPUSH cat1 v1, SymMETAPUSH cat2 v2 => andb (cat1 =? cat2)%N (v1 =? v2)%N
+              | SymOp label1 args1, SymOp label2 args2 =>
+                  if label1 =?i label2 then
+                    match ops label1 with
+                      OpImp _ _ H_Comm _ =>
+                        match (fold_right_two_lists (fun e1 e2 => basic_compare_sstack_val_w_eq_chk_rec ctx e1 e2 maxidx1' sb1' maxidx2' sb2' ops) args1 args2) with
+                        | true => true
+                        | false =>
+                            match H_Comm with
+                            | Some comm_proof =>
+                                match args1, args2 with
+                                | [a1;a2],[b1;b2] =>
+                                    if basic_compare_sstack_val_w_eq_chk_rec ctx a1 b2 maxidx1' sb1' maxidx2' sb2' ops
+                                    then basic_compare_sstack_val_w_eq_chk_rec ctx a2 b1 maxidx1' sb1' maxidx2' sb2' ops
+                                    else false
+                                | _, _ => false
+                                end
+                            | None => false
+                            end
+                        end
+                    end
+                  else false
+              | SymMLOAD soffset1 smem1, SymMLOAD soffset2 smem2 =>
+                  if basic_compare_sstack_val_w_eq_chk smemory_cmp sstorage_cmp sha3_cmp d' ctx soffset1 soffset2 maxidx1' sb1' maxidx2' sb2' ops
+                  then smemory_cmp basic_compare_sstack_val_w_eq_chk_rec ctx smem1 smem2 maxidx1' sb1' maxidx2' sb2' ops
+                  else false
+              | SymSLOAD skey1 sstrg1, SymSLOAD skey2 sstrg2 => 
+                  if basic_compare_sstack_val_w_eq_chk smemory_cmp sstorage_cmp sha3_cmp d' ctx skey1 skey2 maxidx1' sb1' maxidx2' sb2' ops
+                  then sstorage_cmp basic_compare_sstack_val_w_eq_chk_rec ctx sstrg1 sstrg2 maxidx1' sb1' maxidx2' sb2' ops
+                  else false
+              | SymSHA3 soffset1 ssize1 smem1, SymSHA3 soffset2 ssize2 smem2 =>
+                  (* the nested if is to avoid using band *)
+                  if (if basic_compare_sstack_val_w_eq_chk_rec ctx soffset1 soffset2 maxidx1' sb1' maxidx2' sb2' ops then
+                        if basic_compare_sstack_val_w_eq_chk_rec ctx ssize1 ssize2 maxidx1' sb1' maxidx2' sb2' ops then
+                           smemory_cmp basic_compare_sstack_val_w_eq_chk_rec ctx smem1 smem2 maxidx1' sb1' maxidx2' sb2' ops 
+                        else
+                          false
+                      else
+                        false)
+                  then true
+                  else 
+                    sha3_cmp basic_compare_sstack_val_w_eq_chk_rec ctx soffset1 ssize1 smem1 soffset2 ssize2 smem2 maxidx1' sb1' maxidx2' sb2' ops
+              | _, _ => false
+              end
+          end
+      end
+  end.
 
 
 
